simplify example a bit

pulse/share/pulse/examples/EqualOrDisjoint.fst
@@ -37,6 +37,29 @@ let refs_eq_or_disjoint (#a:Type u#a) ([@@@mkey]x1:ref a) ([@@@mkey]x2:ref a) (v
         (x1 |-> Frac 0.5R v1 ** x2 |-> Frac 0.5R v2))
 
 ghost
+fn flip_refs_eq_or_disjoint u#a (#a:Type u#a) ([@@@mkey]x1:ref a) ([@@@mkey]x2:ref a) (v1 v2:a)
+requires refs_eq_or_disjoint x1 x2 v1 v2
+ensures refs_eq_or_disjoint x2 x1 v2 v1
+{
+  unfold refs_eq_or_disjoint;
+  with (eq:bool). assert cond eq _ _;
+
+  let b:bool = reveal eq;
+  if (b)
+  {
+    elim_cond_true _ _ _;
+    intro_cond_true (pure (x2 == x1)) (x2 |-> Frac 0.5R v2 ** x1 |-> Frac 0.5R v1);
+    fold refs_eq_or_disjoint x2 x1 v2 v1;
+  }
+  else
+  {
+    elim_cond_false _ _ _;
+    intro_cond_false (pure (x2 == x1)) (x2 |-> Frac 0.5R v2 ** x1 |-> Frac 0.5R v1);
+    fold refs_eq_or_disjoint x2 x1 v2 v1;
+  }
+}
+
+ghost
 fn intro_refs_eq u#a (#a:Type u#a) (x:ref a) (#v:erased a)
 requires x |-> v
 ensures refs_eq_or_disjoint x x v v
@@ -85,12 +108,12 @@ ensures pure (v1 == v2)
 ghost
 fn get_full_x1 (#a:Type u#0) (x1 x2:ref a) (v1 v2:a)
 requires refs_eq_or_disjoint x1 x2 v1 v2
-ensures
-  x1 |-> v1 ** 
-  (forall* v1'. 
-    (x1 |-> v1') @==> 
-    (exists* v2'. refs_eq_or_disjoint x1 x2 v1' v2' ** 
-        pure (ite (x1==x2) (v2'==v1') (v2'==v2))))
+ensures x1 |-> v1
+ensures pure (x1==x2 ==> v1==v2)
+ensures forall* v1'. 
+  (x1 |-> v1') @==> 
+  (exists* v2'. refs_eq_or_disjoint x1 x2 v1' v2' ** 
+                pure (ite (x1==x2) (v2'==v1') (v2'==v2)))
 { 
   unfold refs_eq_or_disjoint;
   with (eq:bool). assert cond eq _ _;
@@ -144,83 +167,29 @@ ensures
 ghost
 fn get_full_x2 (#a:Type u#0) (x1 x2:ref a) (v1 v2:a)
 requires refs_eq_or_disjoint x1 x2 v1 v2
-ensures
-  x2 |-> v2 ** 
-  (forall* v2'. 
+ensures x2 |-> v2
+ensures pure (x1==x2 ==> v1==v2)
+ensures forall* v2'. 
     (x2 |-> v2') @==> 
     (exists* v1'. refs_eq_or_disjoint x1 x2 v1' v2' ** 
-        pure (ite (x1==x2) (v1'==v2') (v1'==v1))))
+        pure (ite (x1==x2) (v1'==v2') (v1'==v1)))
 {
-  unfold refs_eq_or_disjoint;
-  with (eq:bool). assert cond eq _ _;
-  let v : bool = reveal eq;
-  if (v) 
-  {
-    elim_cond_true _ _ _;
-    rewrite each x1 as x2;
-    gather x2;
-    intro_forall_imp #a
-      (fun v2' -> x2 |-> v2')
-      (fun v2' ->
-        exists* v1'. 
-          refs_eq_or_disjoint x1 x2 v1' v2' **
-          pure (ite (x1==x2) (v1'==v2') (v1'==v1)))
-      emp
-      fn v2' { 
-        share x2;
-        intro_cond_true
-          (pure (x1 == x2))
-          (x1 |-> Frac 0.5R v2' ** x2 |-> Frac 0.5R v2');
-        rewrite (x2 |-> Frac 0.5R v2')
-          as    (x1 |-> Frac 0.5R v2');
-        fold (refs_eq_or_disjoint x1 x2 v2' v2');
-      };
-  }
-  else
-  {
-    elim_cond_false _ _ _;
-    gather x1;
-    gather x2;
-    disjoint_neq x1 x2;
-    intro_forall_imp #a
-      (fun v2' -> x2 |-> v2')
-      (fun v2' ->
-        exists* v1'.
-          refs_eq_or_disjoint x1 x2 v1' v2' **
-          pure (ite (x1==x2) (v1'==v2') (v1'==v1)))
-      (x1 |-> v1)
-      fn v2' { 
-        share x1;
-        share x2;
-        intro_cond_false
-          (pure (x1 == x2))
-          (x1 |-> Frac 0.5R v1 ** x2 |-> Frac 0.5R v2');
-        fold (refs_eq_or_disjoint x1 x2 v1 v2');
-      };
-  }
-}
-
-fn swap (#a:Type0) (x1 x2:ref a) (#v1 #v2:erased a)
-requires refs_eq_or_disjoint x1 x2 v1 v2
-ensures refs_eq_or_disjoint x1 x2 v2 v1
-{
-  if (compare_pointers x1 x2)
-  {
-    elim_is_eq x1 x2;
-  }
-  else
-  {
-    unfold refs_eq_or_disjoint;
-    let u1 = !x1;
-    let u2 = !x2;
-    fold refs_eq_or_disjoint;
-    get_full_x1 _ _ _ _;
-    x1 := u2;
-    elim_forall_imp _ _ _;
-    get_full_x2 _ _ _ _;
-    x2 := u1;
-    elim_forall_imp _ _ _;
-  }
+  flip_refs_eq_or_disjoint _ _ _ _;
+  get_full_x1 _ _ _ _;
+  intro_forall_imp #a
+    (fun v2' -> x2 |-> v2')
+    (fun v2' ->
+      exists* v1'. 
+        refs_eq_or_disjoint x1 x2 v1' v2' **
+        pure (ite (x1==x2) (v1'==v2') (v1'==v1)))
+    (forall* v2'. 
+      (x2 |-> v2') @==> 
+      (exists* v1'. refs_eq_or_disjoint x2 x1 v2' v1' ** 
+          pure (ite (x2==x1) (v1'==v2') (v1'==v1))))
+    fn v2' {
+      elim_forall_imp _ _ v2';
+      flip_refs_eq_or_disjoint x2 x1 _ _ ;
+    };
 }
 
 ghost
@@ -241,7 +210,9 @@ ghost
 fn intro_refs_disj u#a (#a:Type u#a) (x1 x2:ref a) (#v1 #v2:erased a)
 requires x1 |-> v1 ** x2 |-> v2
 ensures refs_eq_or_disjoint x1 x2 v1 v2
+ensures pure (x1 =!= x2)
 {
+  disjoint_neq x1 x2;
   share x1;
   share x2;
   intro_cond_false
@@ -272,6 +243,46 @@ ensures x1 |-> v1 ** x2 |-> v2
   }
 }
 
+
+fn swap (#a:Type0) (x1 x2:ref a) (#v1 #v2:erased a)
+requires refs_eq_or_disjoint x1 x2 v1 v2
+ensures refs_eq_or_disjoint x1 x2 v2 v1
+{
+  if (compare_pointers x1 x2)
+  {
+    elim_is_eq x1 x2;
+  }
+  else
+  {
+    unfold refs_eq_or_disjoint;
+    let u1 = !x1;
+    let u2 = !x2;
+    fold refs_eq_or_disjoint;
+    get_full_x1 _ _ _ _;
+    x1 := u2;
+    elim_forall_imp _ _ _;
+    get_full_x2 _ _ _ _;
+    x2 := u1;
+    elim_forall_imp _ _ _;
+  }
+}
+
+fn swap_unopt (#a:Type0) (x1 x2:ref a) (#v1 #v2:erased a)
+requires refs_eq_or_disjoint x1 x2 v1 v2
+ensures refs_eq_or_disjoint x1 x2 v2 v1
+{
+  unfold refs_eq_or_disjoint;
+  let u1 = !x1;
+  let u2 = !x2;
+  fold refs_eq_or_disjoint;
+  get_full_x1 _ _ _ _;
+  x1 := u2;
+  elim_forall_imp _ _ _;
+  get_full_x2 _ _ _ _;
+  x2 := u1;
+  elim_forall_imp _ _ _;
+}
+
 fn call_swap_eq (#a:Type0) (x:ref a) (#v:erased a)
 requires x |-> v
 ensures x |-> v
@@ -285,7 +296,6 @@ fn call_swap_disj (#a:Type0) (x1 x2:ref a) (#v1 #v2:erased a)
 requires x1 |-> v1 ** x2 |-> v2
 ensures x1 |-> v2 ** x2 |-> v1
 {
-  disjoint_neq x1 x2;
   intro_refs_disj x1 x2;
   swap x1 x2;
   elim_refs_disj  _ _;
